Finish imperative split

BPlusTree_ImpSplit.thy
@@ -1,7 +1,7 @@
-theory BTree_ImpSplit
+theory BPlusTree_ImpSplit
   imports
-    BTree_ImpSet
-    BTree_Split
+    BPlusTree_ImpSet
+    BPlusTree_Split
     Imperative_Loops
 begin
 
@@ -177,6 +177,9 @@ sorted_less xs \<Longrightarrow>
   apply (sep_auto simp add: is_pfa_def)
   done
 
+text "We can fortunately directly use this function as the split_list interpretation"
+
+
 text "Then, using the same loop invariant, a binary split for B-tree-like arrays
 is derived in a straightforward manner."
 
@@ -261,21 +264,13 @@ sorted_less (map snd xs) \<Longrightarrow>
 
 subsection "Refinement of an abstract split"
 
-text "We provide a certain abstract split function
-that is particularly easy to analyse. The idea of this function is due to Peter Lammich."
-
-definition "abs_split xs x = (takeWhile (\<lambda>(_,s). s<x) xs, dropWhile (\<lambda>(_,s). s<x) xs)"
-
-interpretation btree_abs_search: split abs_split
-  unfolding abs_split_def sym[OF linear_split_alt]
-  by unfold_locales
 
 text \<open>Any function that yields the heap rule
 we have obtained for bin\_split and lin\_split also
 refines this abstract split.\<close>
 
-locale imp_split_smeq =
-  fixes split_fun :: "('a::{heap,default,linorder} btnode ref option \<times> 'a) array \<times> nat \<Rightarrow> 'a \<Rightarrow> nat Heap"
+locale imp_split_tree_smeq =
+  fixes split_fun :: "('a::{heap,default,linorder,order_top} btnode ref option \<times> 'a) array \<times> nat \<Rightarrow> 'a \<Rightarrow> nat Heap"
   assumes split_rule: "sorted_less (separators xs) \<Longrightarrow> 
  <is_pfa c xs (a, n)>
    split_fun (a, n) (p::'a)
@@ -286,21 +281,22 @@ locale imp_split_smeq =
 begin
 
 
-lemma abs_split_full: "\<forall>(_,s) \<in> set xs. s < p \<Longrightarrow> abs_split xs p = (xs,[])"
-  by (simp add: abs_split_def)
+lemma linear_split_full: "\<forall>(_,s) \<in> set xs. s < p \<Longrightarrow> linear_split xs p = (xs,[])"
+  by simp
 
 
-lemma abs_split_split:
+lemma linear_split_split:
   assumes "n < length xs" 
     and "(\<forall>(_,s) \<in> set (take n xs). s < p)"
     and " (case (xs!n) of (_,s) \<Rightarrow> \<not>(s < p))"
-  shows "abs_split xs p = (take n xs, drop n xs)"
-  using assms  apply (auto simp add: abs_split_def)
+  shows "linear_split xs p = (take n xs, drop n xs)"
+  using assms  apply (auto)
    apply (metis (mono_tags, lifting) id_take_nth_drop old.prod.case takeWhile_eq_all_conv takeWhile_tail)
   by (metis (no_types, lifting) Cons_nth_drop_Suc case_prod_conv dropWhile.simps(2) dropWhile_append2 id_take_nth_drop)
 
 
-lemma split_rule_abs_split: 
+(* TODO refactor proof? *)
+lemma split_rule_linear_split: 
   shows
     "sorted_less (separators ts) \<Longrightarrow> <
     is_pfa c tsi (a,n)
@@ -309,11 +305,11 @@ lemma split_rule_abs_split:
   <\<lambda>i. 
     is_pfa c tsi (a,n)
     * list_assn (A \<times>\<^sub>a id_assn) ts tsi
-    * \<up>(split_relation ts (abs_split ts p) i)>\<^sub>t"
+    * \<up>(split_relation ts (linear_split ts p) i)>\<^sub>t"
   apply(rule hoare_triple_preI)
   apply (sep_auto heap: split_rule dest!: mod_starD id_assn_list
-      simp add: list_assn_prod_map split_ismeq)
-    apply(auto simp add: is_pfa_def)
+      simp add: list_assn_prod_map split_ismeq simp del: linear_split.simps)
+    apply(auto simp add: is_pfa_def simp del: linear_split.simps)
 proof -
 
   fix h l' assume heap_init:
@@ -323,7 +319,7 @@ proof -
 
 
   show full_thm: "\<forall>j<n. snd (l' ! j) < p \<Longrightarrow>
-       split_relation ts (abs_split ts p) n"
+       split_relation ts (linear_split ts p) n"
   proof -
     assume sm_list: "\<forall>j<n. snd (l' ! j) < p"
     then have "\<forall>j < length (map snd (take n l')). ((map snd (take n l'))!j) < p"
@@ -332,21 +328,21 @@ proof -
       using heap_init by simp
     then have "\<forall>(_,s) \<in> set ts. s < p"
       by (metis case_prod_unfold in_set_conv_nth length_map nth_map)
-    then have "abs_split ts p = (ts, [])"
-      using abs_split_full[of ts p] by simp
-    then show "split_relation ts (abs_split ts p) n"
+    then have "linear_split ts p = (ts, [])"
+      using linear_split_full[of ts p] by simp
+    then show "split_relation ts (linear_split ts p) n"
       using split_relation_length
       by (metis heap_init(2) heap_init(3) length_map length_take min.absorb2)
 
   qed
   then show "\<forall>j<n. snd (l' ! j) < p \<Longrightarrow>
        p \<le> snd (take n l' ! n) \<Longrightarrow>
-       split_relation ts (abs_split ts p) n"
+       split_relation ts (linear_split ts p) n"
     by simp
 
   show part_thm: "\<And>x. x < n \<Longrightarrow>
        \<forall>j<x. snd (l' ! j) < p \<Longrightarrow>
-       p \<le> snd (l' ! x) \<Longrightarrow> split_relation ts (abs_split ts p) x"
+       p \<le> snd (l' ! x) \<Longrightarrow> split_relation ts (linear_split ts p) x"
   proof -
     fix x assume x_sm_len: "x < n"
     moreover assume sm_list: "\<forall>j<x. snd (l' ! j) < p"
@@ -366,20 +362,70 @@ proof -
     then have "case ts!x of (_,s) \<Rightarrow> \<not>(s < p)"
       using heap_init x_sm_len x_sm_len_ts
       by (metis (mono_tags, lifting) case_prod_unfold length_map length_take min.absorb2 nth_take snd_map_help(2))
-    ultimately have "abs_split ts p = (take x ts, drop x ts)"
-      using x_sm_len_ts abs_split_split[of x ts p] heap_init
+    ultimately have "linear_split ts p = (take x ts, drop x ts)"
+      using x_sm_len_ts linear_split_split[of x ts p] heap_init
       by (metis length_map length_take min.absorb2)
-    then show "split_relation ts (abs_split ts p) x"
+    then show "split_relation ts (linear_split ts p) x"
       using x_sm_len_ts 
       by (metis append_take_drop_id heap_init(2) heap_init(3) length_map length_take less_imp_le_nat min.absorb2 split_relation_alt)
   qed
 qed
 
 
-sublocale imp_split abs_split split_fun
+sublocale imp_split_tree linear_split split_fun
   apply(unfold_locales)
-  apply(sep_auto heap: split_rule_abs_split)
+  apply(sep_auto heap: split_rule_linear_split)
   done
+
+end
+
+locale imp_split_list_smeq =
+  fixes split_list_fun :: "('a::{heap,default,linorder,order_top} array \<times> nat) \<Rightarrow> 'a \<Rightarrow> nat Heap"
+  assumes split_list_rule: "sorted_less xs \<Longrightarrow> 
+ <is_pfa c xs (a, n)>
+   split_list_fun (a, n) (p::'a)
+  <\<lambda>r. is_pfa c xs (a, n) *
+                 \<up> (r \<le> n \<and>
+                   (\<forall>j<r. xs ! j < p) \<and>
+                   (r < n \<longrightarrow> p \<le> xs ! r))>\<^sub>t"
+begin
+
+
+lemma split_list_rule_linear_split: 
+  shows
+    "sorted_less ts \<Longrightarrow> <
+    is_pfa c tsi (a,n)
+  * list_assn id_assn ts tsi> 
+    split_list_fun (a,n) p 
+  <\<lambda>i. 
+    is_pfa c tsi (a,n)
+    * list_assn id_assn ts tsi
+    * \<up>(split_relation ts (linear_split_list ts p) i)>\<^sub>t"
+  apply(rule hoare_triple_preI)
+  apply (sep_auto heap: split_list_rule dest!: mod_starD 
+      simp add: list_assn_prod_map split_ismeq id_assn_list_alt simp del: linear_split_list.simps)
+    apply(auto simp add: is_pfa_def split_relation_alt)
+  subgoal by (smt (verit) eq_len_takeWhile_conv leD length_take length_takeWhile_le linorder_neqE_nat min_eq_arg(2) nth_length_takeWhile nth_take nth_take_eq)
+  subgoal by (metis le_neq_implies_less length_take length_takeWhile_le min_eq_arg(2) nth_length_takeWhile nth_take)
+  subgoal 
+    using \<open>\<And>l'a l' bc bb b ac ab aa. \<lbrakk>sorted_less (take n l'a); ts = take n l'a; in_range (ac, bc); \<forall>j<n. l'a ! j < p; (aa, b) \<Turnstile> a \<mapsto>\<^sub>a l'; (ab, bb) \<Turnstile> a \<mapsto>\<^sub>a l'a; c = length l'a; length l' = length l'a; tsi = take n l'a; n \<le> length l'a; take n l' = take n l'a\<rbrakk> \<Longrightarrow> n = length (takeWhile (\<lambda>s. s < p) (take n l'a))\<close> by blast
+  done
+
+
+sublocale imp_split_list linear_split_list split_list_fun
+  apply(unfold_locales)
+  apply(sep_auto heap: split_list_rule_linear_split)
+  done
+
+end
+
+locale imp_split_full_smeq = imp_split_tree_smeq split_fun + imp_split_list_smeq split_list_fun
+  for split_fun:: "('a::{heap,default,linorder,order_top} btnode ref option \<times> 'a) array \<times> nat \<Rightarrow> 'a \<Rightarrow> nat Heap"
+  and split_list_fun :: "('a::{heap,default,linorder,order_top} array \<times> nat) \<Rightarrow> 'a \<Rightarrow> nat Heap"
+begin
+
+sublocale imp_split_full split_fun split_list_fun linear_split linear_split_list
+  by (unfold_locales)
 
 end
 
@@ -389,7 +435,7 @@ text "In order to obtain fully defined functions,
 we need to plug our split function implementations
 into the locales we introduced previously."
 
-interpretation btree_imp_linear_split: imp_split_smeq lin_split
+interpretation btree_imp_linear_split_tree: imp_split_tree_smeq lin_split
   apply unfold_locales
   apply(sep_auto heap: lin_split_rule)
   done
@@ -399,26 +445,117 @@ text "Obtaining actual code turns out to be slightly more difficult
   due to the use of locales. However, we successfully obtain
 the B-tree insertion and membership query with binary search splitting."
 
-global_interpretation btree_imp_binary_split: imp_split_smeq bin_split
-  defines btree_isin = btree_imp_binary_split.isin
-    and btree_ins = btree_imp_binary_split.ins
-    and btree_insert = btree_imp_binary_split.insert
-    and btree_del = btree_imp_binary_split.del
-    and btree_split_max = btree_imp_binary_split.split_max
-    and btree_delete = btree_imp_binary_split.delete
-    and btree_empty = btree_imp_binary_split.empty
+interpretation btree_imp_bin_split_tree: imp_split_tree_smeq bin_split
   apply unfold_locales
   apply(sep_auto heap: bin_split_rule)
   done
 
-declare btree_imp_binary_split.ins.simps[code]
-declare btree_imp_binary_split.isin.simps[code]
-declare btree_imp_binary_split.del.simps[code] btree_imp_binary_split.split_max.simps[code]
+global_interpretation btree_imp_binary_split_list: imp_split_list_smeq bin'_split
+  defines btree_isin_list = btree_imp_binary_split_list.imp_isin_list
+    and btree_ins_list = btree_imp_binary_split_list.imp_ins_list
+    and btree_del_list = btree_imp_binary_split_list.imp_del_list
+  apply unfold_locales
+  apply(sep_auto heap: bin'_split_rule)
+  done
+
+global_interpretation btree_imp_binary_split: imp_split_full_smeq bin_split bin'_split
+  defines btree_isin = btree_imp_binary_split.isin
+    and btree_ins = btree_imp_binary_split.ins
+    and btree_insert = btree_imp_binary_split.insert
+    and btree_del = btree_imp_binary_split.del
+    and btree_delete = btree_imp_binary_split.delete
+    and btree_empty = btree_imp_binary_split.empty
+  apply unfold_locales
+  done
+
+thm btree_imp_binary_split.isin.simps
+lemma [code]: "btree_isin p x =
+!p \<bind>
+(\<lambda>node.
+    case node of
+    Btnode ts t \<Rightarrow>
+      bin_split ts x \<bind>
+      (\<lambda>i. pfa_length ts \<bind>
+            (\<lambda>tsl. if i < tsl
+                    then pfa_get ts i \<bind> (\<lambda>s. let (sub, sep) = s in btree_isin (the sub) x)
+                    else btree_isin t x))
+    | Btleaf xs \<Rightarrow> btree_isin_list x xs)"
+  apply(subst btree_isin_list_def)
+  apply(subst btree_imp_binary_split.isin.simps)
+  by simp
+
+thm btree_imp_binary_split.ins.simps
+lemma [code]: "btree_ins k x p =
+!p \<bind>
+(\<lambda>node.
+    case node of
+    Btnode tsi ti \<Rightarrow>
+      bin_split tsi x \<bind>
+      (\<lambda>i. pfa_length tsi \<bind>
+            (\<lambda>tsl. if i < tsl
+                    then pfa_get tsi i \<bind>
+                         (\<lambda>s. let (sub, sep) = s
+                               in btree_ins k x (the sub) \<bind>
+                                  (\<lambda>r. case r of
+                                        btree_imp_binary_split.T\<^sub>i lp \<Rightarrow>
+                                          pfa_set tsi i (Some lp, sep) \<bind>
+                                          (\<lambda>_. return (btree_imp_binary_split.T\<^sub>i p))
+                                        | btree_imp_binary_split.Up\<^sub>i lp x' rp \<Rightarrow>
+                                            pfa_set tsi i (Some rp, sep) \<bind>
+                                            (\<lambda>_. if tsl < 2 * k
+ then pfa_insert tsi i (Some lp, x') \<bind>
+      (\<lambda>tsi'. p := Btnode tsi' ti \<bind> (\<lambda>_. return (btree_imp_binary_split.T\<^sub>i p)))
+ else pfa_insert_grow tsi i (Some lp, x') \<bind> (\<lambda>tsi'. btree_imp_binary_split.node\<^sub>i k tsi' ti))))
+                    else btree_ins k x ti \<bind>
+                         (\<lambda>r. case r of
+                               btree_imp_binary_split.T\<^sub>i lp \<Rightarrow>
+                                 p := Btnode tsi lp \<bind>
+                                 (\<lambda>_. return (btree_imp_binary_split.T\<^sub>i p))
+                               | btree_imp_binary_split.Up\<^sub>i lp x' rp \<Rightarrow>
+                                   if tsl < 2 * k
+                                   then pfa_append tsi (Some lp, x') \<bind>
+                                        (\<lambda>tsi'.
+                                            p := Btnode tsi' rp \<bind>
+                                            (\<lambda>_. return (btree_imp_binary_split.T\<^sub>i p)))
+                                   else pfa_append_grow' tsi (Some lp, x') \<bind>
+                                        (\<lambda>tsi'. btree_imp_binary_split.node\<^sub>i k tsi' rp))))
+    | Btleaf ksi \<Rightarrow>
+        btree_ins_list x ksi \<bind> btree_imp_binary_split.Lnode\<^sub>i k)"
+  apply(subst btree_ins_list_def)
+  apply(subst btree_imp_binary_split.ins.simps)
+  by simp
+
+thm btree_imp_binary_split.del.simps
+lemma [code]: "btree_del k x tp =
+!tp \<bind>
+(\<lambda>ti. case ti of
+       Btnode tsi tti \<Rightarrow>
+         bin_split tsi x \<bind>
+         (\<lambda>i. pfa_length tsi \<bind>
+               (\<lambda>tsl. if i < tsl
+                       then pfa_get tsi i \<bind>
+                            (\<lambda>(sub, sep).
+                                btree_del k x (the sub) \<bind>
+                                (\<lambda>sub'.
+                                    pfa_set tsi i (Some sub', sep) \<bind>
+                                    (\<lambda>kvs'.
+                                        btree_imp_binary_split.rebalance_middle_tree k kvs' i
+                                         tti \<bind>
+                                        (\<lambda>node'. tp := node' \<bind> (\<lambda>_. return tp)))))
+                       else btree_del k x tti \<bind>
+                            (\<lambda>t'. btree_imp_binary_split.rebalance_last_tree k tsi t' \<bind>
+                                   (\<lambda>node'. tp := node' \<bind> (\<lambda>_. return tp)))))
+       | Btleaf xs \<Rightarrow>
+           btree_del_list x xs \<bind>
+           (\<lambda>xs'. tp := Btleaf xs' \<bind> (\<lambda>_. return tp)))"
+  apply(subst btree_del_list_def)
+  apply(subst btree_imp_binary_split.del.simps)
+  by simp
 
 export_code btree_empty btree_isin btree_insert btree_delete checking OCaml SML Scala
-export_code btree_empty btree_isin btree_insert btree_delete in OCaml module_name BTreeInsert
-export_code btree_empty btree_isin btree_insert btree_delete in SML module_name BTreeInsert
-export_code btree_empty btree_isin btree_insert btree_delete in Scala module_name BTreeInsert
+export_code btree_empty btree_isin btree_insert btree_delete in OCaml module_name BPlusTree
+export_code btree_empty btree_isin btree_insert btree_delete in SML module_name BPlusTree
+export_code btree_empty btree_isin btree_insert btree_delete in Scala module_name BPlusTree
 
 end
 
